src/TypedPackage.v
@@ -1,0 +1,21 @@
+(** This file contains record definitions for
+ ** type, function and predicate environments.
+ **)
+Require Import Expr SepExpr.
+Require Import Env.
+
+Set Implicit Arguments.
+Set Strict Implicit.
+
+Require Import Heaps SepTheoryX.
+
+Module Make (B : Heap) (ST : SepTheoryXType B).
+  Module SEP := SepExpr B ST.
+
+  Record TypeEnv (core : Repr type) (pc st : tvar) : Type :=
+  { Types : Repr type
+  ; Funcs : forall ts, Repr (signature (repr core (repr Types ts)))
+  ; Preds : forall ts, Repr (SEP.ssignature (repr core (repr Types ts)) pc st)
+  }.
+
+End Make.
